michael_formal/drinks_machine.thy
@@ -2,66 +2,50 @@ theory drinks_machine
   imports EFSM
 begin
 
-definition t1_updates :: update_function where
-  "t1_updates = [(''r1'', (V ''i1'')), (''r2'', (N 0))]"
-declare t1_updates_def [simp]
-
 definition t1 :: "transition" where
-"t1 \<equiv> \<lparr> Label = ''select'',
+"t1 \<equiv> \<lparr>
+        Label = ''select'',
         Arity = 1,
-        Guard = trueguard,
-        Outputs = blank,
-        Updates = t1_updates (*<''r1'' := (V ''i1''), ''r2'' := 0>*)
+        Guard = true,
+        Outputs = [],
+        Updates = [(''r1'', (V ''i1'')), (''r2'', (N 0))]
       \<rparr>"
 declare t1_def [simp]
 
-definition t2_updates :: update_function where
-  "t2_updates = [
+definition t2 :: "transition" where
+"t2 \<equiv> \<lparr>
+        Label = ''coin'',
+        Arity = 1,
+        Guard = true,
+        Outputs = [(''o1'', (Plus (V ''r2'') (V ''i1'')))],
+        Updates = [
                   (''r1'', (V ''r1'')),
                   (''r2'', (Plus (V ''r2'') (V ''i1'')))
-                ]"
-declare t2_updates_def [simp]
-
-definition t2_outputs :: output_function where
-  "t2_outputs = [ (''o1'', (Plus (V ''r2'') (V ''i1'')))]"
-declare t2_outputs_def [simp]
-
-definition t2 :: "transition" where
-"t2 \<equiv> \<lparr> Label = ''coin'',
-        Arity = 1,
-        Guard = trueguard,
-        Outputs = t2_outputs,
-        Updates = t2_updates (*<''r1'' := (V ''i1''), ''r2'' := 0>*)
+                ]
       \<rparr>"
 declare t2_def [simp]
 
-definition t3_outputs :: output_function where
-  "t3_outputs = [(''o1'', (V ''r1''))]"
-declare t3_outputs_def [simp]
-
-definition t3_guard :: guard where
-"t3_guard = [(Less (N 100) (V ''r2''))]"
-declare t3_guard_def [simp]
-
 definition t3 :: "transition" where
-"t3 \<equiv> \<lparr> Label = ''vend'',
+"t3 \<equiv> \<lparr>
+        Label = ''vend'',
         Arity = 0,
-        Guard = t3_guard,
-        Outputs = t3_outputs,
-        Updates = no_updates
+        Guard = [((V ''r2'') \<ge> (N 100))],
+        Outputs =  [(''o1'', (V ''r1''))],
+        Updates = [(''r1'', (V ''r1'')), (''r2'', (V ''r2''))]
       \<rparr>"
 declare t3_def [simp]
 
 lemma blank_state : "<> = <''r1'' := 0, ''r2'' := 0>"
   by (metis fun_upd_triv null_state_def)
 
-lemma blank_state2 (*[intro]*):
+lemma blank_state2:
   assumes "P <''r1'' := 0, ''r2'' := 0>"
   shows "P <>"
   by (metis assms blank_state)
 
 definition vend :: "efsm" where
-"vend \<equiv> \<lparr> S = [1,2,3],
+"vend \<equiv> \<lparr> 
+          S = [1,2,3],
           s0 = 1,
           T = \<lambda> (a,b) .
               if (a,b) = (1,2) then [t1]
@@ -77,13 +61,13 @@ lemma "observe_trace vend (s0 vend) <> [] = []"
 lemma "observe_trace vend (s0 vend) <> [(''select'', [1])] = [[]]"
   by simp
 
-lemma [intro]: "observe_trace vend (s0 vend) <> [(''select'', [1]), (''coin'', [50])] = [[], [50]]"
+lemma "observe_trace vend (s0 vend) <> [(''select'', [1]), (''coin'', [50])] = [[], [50]]"
   by (simp_all add: showsp_int_def showsp_nat.simps shows_string_def null_state_def)
 
-lemma [intro]: "observe_trace vend (s0 vend) <> [(''select'', [1]), (''coin'', [50]), (''coin'', [51])] = [[], [50], [101]]"
+lemma "observe_trace vend (s0 vend) <> [(''select'', [1]), (''coin'', [50]), (''coin'', [50])] = [[], [50], [100]]"
   by (simp add: showsp_int_def showsp_nat.simps shows_string_def null_state_def)
 
-lemma "observe_trace vend (s0 vend) <> [(''select'', [1]), (''coin'', [50]), (''coin'', [51]), (''vend'', [])] = [[], [50], [101], [1]]"
+lemma "observe_trace vend (s0 vend) <> [(''select'', [1]), (''coin'', [50]), (''coin'', [50]), (''vend'', [])] = [[], [50], [100], [1]]"
   by (simp add: showsp_int_def showsp_nat.simps shows_string_def null_state_def)
 
 (*Stop when we hit a spurious input*)
@@ -92,4 +76,16 @@ lemma "observe_trace vend (s0 vend) <> [(''select'', [1]), (''cat'', [50])] = [[
 
 lemma "observe_trace vend (s0 vend) <> [(''select'', [1]), (''cat'', [50]), (''coin'', [50])] = [[]]"
   by simp
+
+(*This crashes because of showsp_nat.simps*)
+(*What is ".simps"? Why not "showsp_nat_def"?*)
+(*lemma "observe_registers vend (s0 vend) <> [(''select'', [1]), (''coin'', [50]), (''coin'', [51])] = <''r1'':=1, ''r2'':=101>"
+  apply (simp add: showsp_int_def showsp_nat.simps shows_string_def null_state_def)*)
+
+
+lemma "((observe_trace e (s0 e) <> t) = obs) \<longrightarrow> ((observe_trace e (s0 e) <> (t@t')) = obs@(observe_trace e (s0 e) (observe_registers e (s0 e) <> t) t'))"
+  apply (induct_tac "t")
+   apply (simp)
+  apply (simp only: observe_registers_def)
+  sorry
 end
