michael_formal/Syntax.thy
@@ -1,0 +1,21 @@
+theory Syntax
+imports "~~/src/HOL/IMP/Hoare" types
+begin
+
+definition Geq :: "aexp \<Rightarrow> aexp \<Rightarrow> bexp" (infix "\<ge>" 60) where
+  "Geq a b  = (Not (Less a b))"
+declare Geq_def [simp]
+
+definition Gt :: "aexp \<Rightarrow> aexp \<Rightarrow> bexp" (infix ">" 60) where
+  "Gt a b = (Less b a)"
+declare Gt_def [simp]
+
+definition Leq :: "aexp \<Rightarrow> aexp \<Rightarrow> bexp" (infix "\<le>" 60) where
+  "Leq a b = (Not (Gt a b))"
+declare Leq_def [simp]
+
+definition true :: guard  where
+  "true = [(Bc True)]"
+declare true_def [simp]
+
+end
